WIP: test theta on iter

iodiv/DivFreeTauDM.Test.fst
@@ -18,15 +18,20 @@ let th #a = theta #a #io_sig iodiv_act
 
 let test1 (fd:file_descr) : Lemma (th (body1 fd) `ile` ibody1 fd) = ()
 
-
+#set-options "--split_queries always"
 let test2 (fd:file_descr) =
+  let body' = lift_body (ibody1 fd) in
 //  pre1_inv1 fd;
-  let body' = lift_body #file_descr (ibody1 fd) #unit in
 //  let body_inv = repeat_body_inv #unit (fun _ -> pre1 fd) (inv1 fd) in
-//  repeat_inv_proof #unit (fun _ -> (pre1 fd)) (inv1 fd) () ;
-//  i_iter_mono (fun _ -> repeat_body_inv (fun _ -> (pre1 fd)) (inv1 fd) ()) (repeat_body_inv (fun _ -> (pre1 fd)) (inv1 fd)) () ;
 
   test1 fd;
-  assume (th (loop1 fd) `ile` i_iter body' ());
+
+  assert (th (m_bind (body1 fd) (fun msg -> m_ret (Inl ()))) `ile` i_bind #_ #(either unit string) (ibody1 fd) (fun _ -> i_ret (Inl ())));
+  assert (th (m_bind (body1 fd) (fun msg -> m_ret (Inl ()))) `ile` lift_body (ibody1 fd) ());
+  //repeat_inv_proof #unit (fun _ -> (pre1 fd)) (inv1 fd) () ;
+  //i_iter_mono (fun _ -> repeat_body_inv (fun _ -> (pre1 fd)) (inv1 fd) ()) (repeat_body_inv (fun _ -> (pre1 fd)) (inv1 fd)) () ;
+  assume (th (m_iter (fun i -> m_bind (body1 fd) (fun msg -> m_ret (Inl i))) ()) `ile` i_iter (lift_body (ibody1 fd)) ());
+  assert (th (m_iter (body1' fd) ()) `ile` i_iter body' ());
+  assert (th (loop1 fd) `ile` i_iter body' ());
   itest1 fd;
   assert (th (loop1 fd) `ile` iloop1 fd)
